最终版

strat_liquidity/examples/honeypots/Honeypots.v
@@ -126,7 +126,7 @@ Section Gift1ETH.
         let amt := st.(balance) in
         Ok ( st <| balance := 0 |> , [ act_transfer (ctx_from ctx) amt ] )
       else
-        Ok (st, [])
+        Err default_error
     else
       Err default_error.
 
@@ -138,7 +138,7 @@ Section Gift1ETH.
     if (require_zero ctx) then
       if (h =? st.(hashPass))%N 
       then Ok (st <| passHasBeenSet := true |>, [])
-      else Ok (st, [])
+      else Err default_error
     else
       Err default_error.
 
@@ -294,38 +294,70 @@ Section Liqiuidity.
 
   Hypothesis attacker_eoa : address_not_contract attacker = true.
   Hypothesis honest_eoa : address_not_contract honest = true.
+  Hypothesis H_honest_bal_ge_1 : forall (s:ChainState), (funds s honest >= 1)%Z.
+
+  Hypothesis H_attack_bal_ge_1 : forall (s:ChainState), (funds s attacker >= 1)%Z.
 
   Variable attacker_pass : N.
 
   Variable honest_pass : N.
 
+  Hypothesis pass_neq : attacker_pass <> honest_pass.
+
+  Hypothesis honest_pass_neq : (sha3 honest_pass <> 0)%N.
+  Hypothesis attacker_pass_neq : (sha3 attacker_pass <> 0)%N.
+
+  Section sha3_coorect.
+
+  Lemma pos_inj : forall p q : positive, N.pos p = N.pos q -> p = q.
+  Proof.
+    intros p q H. inversion H. reflexivity.
+  Qed.
+
+    
+  Require  Coq.NArith.NArith.
+  Require  stdpp.countable.
+
+
+  Lemma sha3_pass_neq :sha3 attacker_pass <> sha3 honest_pass.
+  Proof.
+    intros H.
+    eauto.
+    
+    unfold sha3.
+    apply pos_inj in H.
+    eapply stdpp.countable.encode_inj in H.
+    unfold countable.encode in H.
+    simpl in H.
+    intuition.
+  Qed.
+
+  End sha3_coorect.
+
   Definition attacker_call_SetPass (state : State): Action :=
     build_call attacker caddr 1 (SetPass (sha3 attacker_pass)).
+
+  Definition attacker_call_PassHasBeenSetMsg (state : State): Action :=
+    build_call attacker caddr 0 (PassHasBeenSetMsg (sha3 attacker_pass)).
 
   Definition honest_call_SetPass (state : State): Action :=
     build_call honest caddr 1 (SetPass (sha3 honest_pass)).
 
-  (* Definition m := (sha3 2%N).
+  Definition honest_call_GetGift (state : State): Action :=
+    build_call honest caddr 0 (GetGift honest_pass).
 
-  Definition pass := 2%N.
-  
-  Goal m = sha3 pass.
-  Proof.
-    unfold m.
-    unfold pass.
-    eauto.
-  Qed.  *)
-
-  Definition honest_call_getGift (state : State): Action :=
-    build_call honest caddr 1 (GetGift honest_pass).
+  Definition honest_call_PassHasBeenSetMsg  (state : State): Action :=
+      build_call honest caddr 0 (PassHasBeenSetMsg  (sha3 honest_pass)).
 
   Definition attacker_strat : (strat miner [attacker]) :=
     fun s0 s tr =>
       match get_contract_state s caddr with
       | Some state =>
-          if ((state.(hashPass) =? 0)%N) then
+          if ((state.(hashPass) =? sha3 attacker_pass)%N) then
+            [attacker_call_PassHasBeenSetMsg state]
+          else if (negb state.(passHasBeenSet)) then
             [attacker_call_SetPass state]
-          else
+          else 
             []
       | None => []
       end.
@@ -334,7 +366,7 @@ Section Liqiuidity.
     fun s0 s tr =>
       match get_contract_state s caddr with
       | Some state =>
-        [honest_call_SetPass state;honest_call_getGift state]
+        [honest_call_SetPass state;honest_call_GetGift state;honest_call_PassHasBeenSetMsg state]
       | None => []
       end.
 
@@ -389,19 +421,11 @@ Section Liqiuidity.
         propify.
         unfold require_zero in Ezero.
         lia.
-        inversion receive_some. simpl.
-        propify.
-        unfold require_zero in Ezero.
-        intuition.
       + reduce_passHasBeenSet_fn. cbn in *.
         inversion receive_some. simpl.
         unfold require_zero in Ezero.
         propify.
         lia.
-        inversion receive_some. simpl.
-        unfold require_zero in Ezero.
-        propify.
-        intuition.
       + inversion receive_some. simpl.
         propify.
         lia.
@@ -425,23 +449,11 @@ Section Liqiuidity.
         propify.
         unfold require_zero in Ezero.
         inversion receive_some; destruct head; cbn in *; lia.
-        inversion receive_some. simpl.
-        propify.
-        unfold require_zero in Ezero.
-        inversion receive_some; destruct head; cbn in *; try lia.
-        intuition.
-        intuition.
       + reduce_passHasBeenSet_fn. cbn in *.
         inversion receive_some. simpl.
         unfold require_zero in Ezero.
         propify.
         inversion receive_some; destruct head; cbn in *; try lia.
-        inversion receive_some. simpl.
-        unfold require_zero in Ezero.
-        propify.
-        inversion receive_some; destruct head; cbn in *; try lia.
-        intuition.
-        intuition.
       + inversion receive_some. simpl.
         propify.
         inversion receive_some; destruct head; cbn in *; lia.
@@ -502,6 +514,52 @@ Section Liqiuidity.
   Proof.
     unfold is_call_act.
     unfold user_call_GetGift.
+    simpl.
+    destruct_address_eq;eauto.
+  Qed.
+
+  Lemma honest_call_GetGift_is_call_act cstate:
+    is_call_act (honest_call_GetGift cstate) = true .
+  Proof.
+    unfold is_call_act.
+    unfold honest_call_GetGift.
+    simpl.
+    destruct_address_eq;eauto.
+  Qed.
+
+  Lemma attacker_call_SetPass_is_call_act cstate:
+    is_call_act (attacker_call_SetPass cstate) = true .
+  Proof.
+    unfold is_call_act.
+    unfold attacker_call_SetPass.
+    simpl.
+    destruct_address_eq;eauto.
+  Qed.
+
+  Lemma attacker_call_PassHasBeenSetMsg_is_call_act cstate:
+    is_call_act (attacker_call_PassHasBeenSetMsg cstate) = true .
+  Proof.
+    unfold is_call_act.
+    unfold attacker_call_PassHasBeenSetMsg.
+    simpl.
+    destruct_address_eq;eauto.
+  Qed.
+
+  
+  Lemma honest_call_SetPass_is_call_act cstate:
+    is_call_act (honest_call_SetPass cstate) = true .
+  Proof.
+    unfold is_call_act.
+    unfold honest_call_SetPass.
+    simpl.
+    destruct_address_eq;eauto.
+  Qed.
+
+  Lemma honest_call_PassHasBeenSetMsg_is_call_act cstate:
+    is_call_act ( honest_call_PassHasBeenSetMsg cstate) = true .
+  Proof.
+    unfold is_call_act.
+    unfold honest_call_PassHasBeenSetMsg.
     simpl.
     destruct_address_eq;eauto.
   Qed.
@@ -1039,12 +1097,14 @@ Section Liqiuidity.
     intuition.
     specialize (hashPass_kown_all_state s cstate Hcs_s ).
     propify.
-    inversion Hcstate_s_t0;subst.
-    intuition.
-    (* caddr = miner *)
     eapply address_not_contract_negb in user1_eoa.
     rewrite e in *.
     intuition.
+
+    (* caddr = miner *)
+    (* eapply address_not_contract_negb in user1_eoa.
+    rewrite e in *.
+    intuition. *)
     (* 
       n: sender cstate <> miner
       n0: caddr <> sender cstate
@@ -1259,10 +1319,6 @@ Section Liqiuidity.
     simpl.
     eauto.
     intuition.
-    specialize (hashPass_kown_all_state s cstate Hcs_s ).
-    propify.
-    inversion Hcstate_s_t0;subst.
-    intuition.
   Qed.
 
   Lemma honeypot_satisfy_base_liquidity:
@@ -1349,5 +1405,2313 @@ Section Liqiuidity.
     eauto.
   Qed.
 
+  Lemma honest_call_GetGift_is_call_act_transition_correct_nopass:
+  forall (s:ChainState) cstate,
+    contract_state s caddr = Some cstate ->
+    transition_reachable miner contract caddr s0 s ->
+    cstate.(passHasBeenSet) = true ->
+    cstate.(hashPass) <> sha3 honest_pass ->
+    transition miner s (honest_call_GetGift cstate) = Err StratModel.default_error.
+  Proof.
+    intros * Hcs_s Htrc_s H_passB H_neq.
+    unfold transition.
+    unfold queue_isb_empty.
+    eapply transition_reachable_queue_is_empty in Htrc_s as Hqueue_s;eauto.
+    rewrite Hqueue_s.
+    rewrite honest_call_GetGift_is_call_act.
+    unfold evaluate_action.
+    rewrite get_valid_header_is_valid_header.
+    unfold user_call_GetGift .
+    simpl.
+    destruct_address_eq;try congruence.
+    simpl.
+    assert (Hec_s:env_contracts s caddr = Some (contract:WeakContract)).
+    {
+      eapply transition_reachable_impl_reachable_through in Htrc_s.
+      eapply reachable_through_contract_deployed in Htrc_s;eauto.
+      decompose_is_init_state H_init.
+      eauto.
+      eauto.
+    }
+    eapply address_not_contract_negb in honest_eoa.
+    rewrite honest_eoa.
+    unfold send_or_call.
+    simpl.
+    assert( H_caddr_not_EOA : address_is_contract caddr = true).
+    {
+      eapply contract_addr_format in Hec_s;eauto.
+      eapply transition_reachable_impl_reachable in Htrc_s;eauto.  
+    }
+    assert(Hrc_s:reachable s).
+    {
+      eapply transition_reachable_impl_reachable in Htrc_s;eauto.
+    }
+    assert(Hbal:env_account_balances s caddr = cstate.(balance)).
+    {
+      eapply balance_on_chain_forall;eauto.
+      unfold outgoing_acts.
+      rewrite Hqueue_s.
+      simpl.
+      eauto.
+    }
+    destruct_address_eq;try congruence.
+    + assert ((0 >? miner_reward + env_account_balances s honest )%Z 
+                = false).
+      {
+        unfold miner_reward.
+        eapply (account_balance_nonnegative s honest) in Hrc_s.
+        lia.
+      }
+      rewrite H.
+      rewrite Hec_s.
+      unfold contract_state in Hcs_s.
+      simpl in Hcs_s.
+      destruct (env_contract_states s caddr) eqn : Hecs_s;try congruence.
+      simpl.
+      rewrite Hcs_s.
+      simpl.
+      setoid_rewrite deserialize_serialize.
+      simpl.
+      cbn in *.
+      unfold receive.
+      simpl.
+      simpl.
+      destruct (hashPass cstate =? sha3 honest_pass)%N eqn : N.
+      - propify. intuition.
+      - propify. 
+        simpl.
+        
+        eauto.
+    + assert ((0 >?  env_account_balances s honest )%Z 
+                = false).
+      {
+        unfold miner_reward.
+        eapply (account_balance_nonnegative s honest) in Hrc_s.
+        lia.
+      }
+      rewrite H.
+      rewrite Hec_s.
+      unfold contract_state in Hcs_s.
+      simpl in Hcs_s.
+      destruct (env_contract_states s caddr) eqn : Hecs_s;try congruence.
+      simpl.
+      rewrite Hcs_s.
+      simpl.
+      setoid_rewrite deserialize_serialize.
+      simpl.
+      cbn in *.
+      unfold receive.
+      simpl.
+      unfold address_not_contract.
+      destruct (hashPass cstate =? sha3 honest_pass)%N eqn : N.
+      - propify. intuition.
+      - propify. 
+        simpl.
+        
+        eauto.
+    + assert ((0 >?  env_account_balances s honest )%Z 
+                = false).
+      {
+        unfold miner_reward.
+        eapply (account_balance_nonnegative s honest) in Hrc_s.
+        lia.
+      }
+      rewrite H.
+      rewrite Hec_s.
+      unfold contract_state in Hcs_s.
+      simpl in Hcs_s.
+      destruct (env_contract_states s caddr) eqn : Hecs_s;try congruence.
+      simpl.
+      rewrite Hcs_s.
+      simpl.
+      setoid_rewrite deserialize_serialize.
+      simpl.
+      cbn in *.
+      unfold receive.
+      simpl.
+      unfold address_not_contract.
+      destruct (hashPass cstate =? sha3 honest_pass)%N eqn : N.
+      - propify. intuition.
+      - propify. 
+        simpl.
+        eauto.
+  Qed.
+
+  Lemma honest_call_SetPass_is_call_act_transition_correct_nopass:
+    forall (s:ChainState) cstate,
+      contract_state s caddr = Some cstate ->
+      transition_reachable miner contract caddr s0 s ->
+      cstate.(passHasBeenSet) = true ->
+      cstate.(hashPass) <> sha3 honest_pass ->
+      exists s',
+      transition miner s (honest_call_SetPass cstate) = Ok s'.
+  Proof.
+    intros * Hcs_s Htrc_s H_passB H_pass .
+    eexists.
+    unfold transition.
+    unfold queue_isb_empty.
+    eapply transition_reachable_queue_is_empty in Htrc_s as Hqueue_s;eauto.
+    rewrite Hqueue_s.
+    rewrite honest_call_SetPass_is_call_act.
+    unfold evaluate_action.
+    rewrite get_valid_header_is_valid_header.
+    unfold user_call_GetGift .
+    simpl.
+    destruct_address_eq;try congruence.
+    simpl.
+    assert (Hec_s:env_contracts s caddr = Some (contract:WeakContract)).
+    {
+      eapply transition_reachable_impl_reachable_through in Htrc_s.
+      eapply reachable_through_contract_deployed in Htrc_s;eauto.
+      decompose_is_init_state H_init.
+      eauto.
+      eauto.
+    }
+    eapply address_not_contract_negb in honest_eoa.
+    rewrite honest_eoa.
+    unfold send_or_call.
+    simpl.
+    assert( H_caddr_not_EOA : address_is_contract caddr = true).
+    {
+      eapply contract_addr_format in Hec_s;eauto.
+      eapply transition_reachable_impl_reachable in Htrc_s;eauto.  
+    }
+    assert(Hrc_s:reachable s).
+    {
+      eapply transition_reachable_impl_reachable in Htrc_s;eauto.
+    }
+    assert(Hbal:env_account_balances s caddr = cstate.(balance)).
+    {
+      eapply balance_on_chain_forall;eauto.
+      unfold outgoing_acts.
+      rewrite Hqueue_s.
+      simpl.
+      eauto.
+    }
+    destruct_address_eq;try congruence.
+    + assert ((1 >? miner_reward + env_account_balances s honest )%Z 
+                = false).
+      {
+        unfold miner_reward.
+        eapply (account_balance_nonnegative s honest) in Hrc_s.
+        lia.
+      }
+      rewrite H.
+      rewrite Hec_s.
+      unfold contract_state in Hcs_s.
+      simpl in Hcs_s.
+      destruct (env_contract_states s caddr) eqn : Hecs_s;try congruence.
+      simpl.
+      rewrite Hcs_s.
+      simpl.
+      setoid_rewrite deserialize_serialize.
+      simpl.
+      cbn in *.
+      unfold receive.
+      simpl.
+      unfold address_not_contract.
+      destruct (hashPass cstate =? sha3 honest_pass)%N eqn : N.
+      - propify. intuition.
+      - propify. 
+        simpl.
+        unfold  setPass.
+        simpl.
+        rewrite H_passB.
+        unfold  one_ether.
+        simpl.
+        eauto.
+      
+    + eapply address_not_contract_negb in H_miner.
+      rewrite e1 in *.
+      intuition.
+    + assert ((1 >?  env_account_balances s honest )%Z 
+                = false).
+      {
+        unfold miner_reward.
+        eapply (account_balance_nonnegative s honest) in Hrc_s.
+        specialize (H_honest_bal_ge_1 s).
+        unfold funds in *.
+
+        lia.
+      }
+      rewrite H.
+      rewrite Hec_s.
+      unfold contract_state in Hcs_s.
+      simpl in Hcs_s.
+      destruct (env_contract_states s caddr) eqn : Hecs_s;try congruence.
+      simpl.
+      rewrite Hcs_s.
+      simpl.
+      setoid_rewrite deserialize_serialize.
+      simpl.
+      cbn in *.
+      unfold receive.
+      simpl.
+      unfold address_not_contract.
+      destruct (hashPass cstate =? sha3 honest_pass)%N eqn : N.
+      - propify. intuition.
+      - propify. 
+        simpl.
+        unfold  setPass.
+        simpl.
+        rewrite H_passB.
+        unfold  one_ether.
+        simpl.
+        eauto.
+  Qed.
+
+  Lemma honest_call_SetPass_is_call_act_state_correct:
+  forall (s s':ChainState) cstate,
+     contract_state s caddr = Some cstate ->
+     transition_reachable miner contract caddr s0 s ->
+     transition miner s (honest_call_SetPass cstate) = Ok s' ->
+     funds s' caddr  >= funds s caddr.
+ Proof.
+   intros * Hcs_s Htrc_s Htrans.
+   eapply transition_reachable_queue_is_empty in Htrc_s as Hqueue_s;eauto.
+   assert (Hact_call : is_call_act ((honest_call_SetPass cstate)) = true).
+   {
+     unfold is_call_act.
+     unfold honest_call_SetPass.
+     unfold build_call.
+     destruct_address_eq;eauto.
+   }
+   assert(ttrace_s_s : TransitionTrace miner s s) by eapply clnil.
+   assert(ttrace_s_s' : TransitionTrace miner s s').
+   {
+     econstructor;eauto.
+     eapply step_trans;eauto.
+
+   }
+   assert(Htrct_s_s' : reachable_via miner contract caddr s0 s s').
+   {
+     econstructor;eauto.
+   }
+   assert(Hrt : reachable_through s s').
+   {
+     eapply reachable_via_impl_reachable_through in Htrct_s_s';eauto.
+   }
+   assert(H_t: reachable s') by eauto.
+   destruct H_t as [trace].
+   assert (Hec_s : env_contracts s caddr = Some ((contract : WeakContract))).
+   {
+     pose proof H_init.
+     decompose_is_init_state H_init.
+     eapply reachable_through_contract_deployed in H_env_contracts.
+     eauto.
+     eapply transition_reachable_impl_reachable_through in Htrc_s;eauto.
+   }
+   assert (Hec_s' : env_contracts s' caddr = Some ((contract : WeakContract))).
+   {
+     pose proof H_init.
+     decompose_is_init_state H_init.
+     eapply reachable_through_contract_deployed in H_env_contracts.
+     eauto.
+     eapply transition_reachable_impl_reachable_through in Htrc_s;eauto.
+   }
+   eapply deployed_contract_state_typed in Hec_s';eauto.
+   destruct Hec_s' as [cstate_s' Hcs_s'].
+
+   eauto.
+   unfold transition in Htrans.
+   unfold queue_isb_empty in Htrans.
+   rewrite Hqueue_s in Htrans.
+   rewrite Hact_call in Htrans.
+   destruct (evaluate_action true s (get_valid_header miner s)
+   [honest_call_SetPass cstate ]) eqn : H_exec;try congruence.
+   unfold evaluate_action in H_exec.
+   rewrite get_valid_header_is_valid_header in H_exec.
+   destruct (find_origin_neq_from [honest_call_SetPass cstate]) ; try congruence.
+   destruct (find_invalid_root_action [honest_call_SetPass cstate]);try congruence.
+   set (mid_state := {|
+     chain_state_env := add_new_block_to_env (get_valid_header miner s) s;
+     chain_state_queue := [user_call_GetGift cstate]
+   |}) in H_exec.
+   simpl in *.
+   destruct_address_eq;try congruence.
+   simpl in *.
+   destruct(send_or_call honest honest caddr 1
+   (Some (serialize (SetPass (sha3 honest_pass))))
+   (add_new_block_to_env (get_valid_header miner s) s)) eqn : H_send_or_call_GetGift;try congruence.
+   unfold send_or_call in  H_send_or_call_GetGift.
+   simpl in H_send_or_call_GetGift.
+   eapply address_not_contract_negb in H_miner.
+   assert( H_caddr_not_EOA : address_is_contract caddr = true).
+   {
+     eapply contract_addr_format in Hec_s;eauto.
+     eapply transition_reachable_impl_reachable in Htrc_s;eauto.  
+   }
+   destruct_address_eq;simpl in *;try congruence.
+   
+   (* 
+     e: sender cstate = miner
+     n: caddr <> sender cstate
+     e0: caddr = caddr
+     n0: caddr <> miner 
+   *)
+   destruct(1 >? miner_reward + env_account_balances s honest)%Z;try congruence.
+   rewrite Hec_s in H_send_or_call_GetGift.
+   assert(Hcstate_s_t0:contract_state s caddr = Some cstate) by eauto.
+   unfold contract_state in Hcstate_s_t0.
+   simpl in Hcstate_s_t0.
+   destruct (env_contract_states s caddr) eqn : Hcstate_s_t0';try congruence.
+   destruct (weak_error_to_error_receive
+   (wc_receive contract
+      (s <| chain_height := S (chain_height s) |> <|
+       current_slot := (current_slot s + 1)%nat |> <|
+       finalized_height := finalized_height s |>)
+      {|
+        ctx_origin := honest;
+        ctx_from := honest;
+        ctx_contract_address := caddr;
+        ctx_contract_balance :=
+          1 + env_account_balances s caddr;
+        ctx_amount := 1
+      |} s1
+      (Some (serialize (SetPass (sha3 honest_pass)))))) eqn : H_wc_receive_s1;try congruence.
+   unfold weak_error_to_error_receive in H_wc_receive_s1.
+   unfold bind_error in H_wc_receive_s1.
+   destruct (wc_receive contract
+   (s <| chain_height := S (chain_height s) |> <| current_slot
+    := (current_slot s + 1)%nat |> <| finalized_height :=
+    finalized_height s |>)
+   {|
+     ctx_origin := honest;
+     ctx_from := honest;
+     ctx_contract_address := caddr;
+     ctx_contract_balance := 1 + env_account_balances s caddr;
+     ctx_amount := 1
+   |} s1 (Some (serialize (SetPass (sha3 honest_pass)))))
+     eqn : H_wc_receive_s1';try congruence.
+   
+   set (cchain := s <| chain_height := S (chain_height s) |> <| current_slot :=
+   (current_slot s + 1)%nat |> <| finalized_height :=
+   finalized_height s |>) in H_wc_receive_s1'.
+   set (cctx := {|
+   ctx_origin := honest;
+   ctx_from := honest;
+   ctx_contract_address := caddr;
+   ctx_contract_balance := 1 + env_account_balances s caddr;
+   ctx_amount := 1
+  |}) in H_wc_receive_s1'.
+   
+   destruct t2 as [new_state new_acts].
+
+   destruct (wc_receive_strong ltac:(try eassumption))
+   as (prev_state_strong & msg_strong & resp_state_strong &
+     deser_state & deser_msg & <- & receive).
+
+   simpl in deser_msg.
+   destruct (msg_strong) eqn : H_msg;try congruence.
+   rewrite deserialize_serialize in deser_msg.
+   rewrite <- deser_msg in receive.
+   rewrite deser_state in Hcstate_s_t0.
+   simpl in receive.
+   rename receive into receive_some.
+   unfold receive in receive_some.
+   reduce_setPass.
+   propify.
+   destruct_and_split.
+
+   (* 111 *)
+   inversion receive_some.
+   subst.
+   inversion H_wc_receive_s1;subst.
+   inversion H_send_or_call_GetGift;subst.
+   simpl in H_exec.
+   inversion H_exec;subst.
+   inversion Htrans;subst.
+   simpl.
+   unfold funds.
+   simpl.
+   destruct_address_eq;try congruence.
+   lia.
+
+   inversion receive_some.
+   subst.
+   inversion H_wc_receive_s1;subst.
+   inversion H_send_or_call_GetGift;subst.
+   simpl in H_exec.
+   inversion H_exec;subst.
+   inversion Htrans;subst.
+   simpl.
+   unfold funds.
+   simpl.
+   destruct_address_eq;try congruence.
+   lia.
+   
+
+   (* caddr = miner *)
+   eapply address_not_contract_negb in honest_eoa.
+   rewrite e in *.
+   intuition.
+   (* 
+     n: sender cstate <> miner
+     n0: caddr <> sender cstate
+     e: caddr = caddr
+     n1: caddr <> miner
+   *)
+   destruct(1 >? env_account_balances s honest)%Z;try congruence.
+   rewrite Hec_s in H_send_or_call_GetGift.
+   assert(Hcstate_s_t0:contract_state s caddr = Some cstate) by eauto.
+   unfold contract_state in Hcstate_s_t0.
+   simpl in Hcstate_s_t0.
+   destruct (env_contract_states s caddr) eqn : Hcstate_s_t0';try congruence.
+   destruct (weak_error_to_error_receive
+   (wc_receive contract
+      (s <| chain_height := S (chain_height s) |> <|
+       current_slot := (current_slot s + 1)%nat |> <|
+       finalized_height := finalized_height s |>)
+      {|
+        ctx_origin := honest;
+        ctx_from := honest;
+        ctx_contract_address := caddr;
+        ctx_contract_balance :=
+          1 + env_account_balances s caddr;
+        ctx_amount := 1
+      |} s1
+      (Some (serialize (SetPass (sha3 honest_pass)))))) eqn : H_wc_receive_s1;try congruence.
+   unfold weak_error_to_error_receive in H_wc_receive_s1.
+   unfold bind_error in H_wc_receive_s1.
+   destruct (wc_receive contract
+   (s <| chain_height := S (chain_height s) |> <| current_slot
+    := (current_slot s + 1)%nat |> <| finalized_height :=
+    finalized_height s |>)
+   {|
+     ctx_origin := honest;
+     ctx_from := honest;
+     ctx_contract_address := caddr;
+     ctx_contract_balance := 1 + env_account_balances s caddr;
+     ctx_amount := 1
+   |} s1 (Some (serialize (SetPass (sha3 honest_pass)))))
+     eqn : H_wc_receive_s1';try congruence.
+   
+   set (cchain := s <| chain_height := S (chain_height s) |> <| current_slot
+   := (current_slot s + 1)%nat |> <| finalized_height :=
+   finalized_height s |>) in H_wc_receive_s1'.
+   set (cctx := {|
+   ctx_origin := honest;
+   ctx_from := honest;
+   ctx_contract_address := caddr;
+   ctx_contract_balance := 1 + env_account_balances s caddr;
+   ctx_amount := 1
+  |}) in H_wc_receive_s1'.
+   
+   destruct t2 as [new_state new_acts].
+
+   destruct (wc_receive_strong ltac:(try eassumption))
+   as (prev_state_strong & msg_strong & resp_state_strong &
+     deser_state & deser_msg & <- & receive).
+
+   simpl in deser_msg.
+   destruct (msg_strong) eqn : H_msg;try congruence.
+   rewrite deserialize_serialize in deser_msg.
+   rewrite <- deser_msg in receive.
+   rewrite deser_state in Hcstate_s_t0.
+   simpl in receive.
+   rename receive into receive_some.
+   unfold receive in receive_some.
+   reduce_setPass.
+   (* 111 *)
+   inversion receive_some.
+   subst.
+   inversion H_wc_receive_s1;subst.
+   inversion H_send_or_call_GetGift;subst.
+   simpl in H_exec.
+   inversion H_exec;subst.
+   inversion Htrans;subst.
+   simpl.
+   unfold funds.
+   simpl.
+   destruct_address_eq;try congruence.
+   lia.
+
+   inversion receive_some.
+   subst.
+   inversion H_wc_receive_s1;subst.
+   inversion H_send_or_call_GetGift;subst.
+   simpl in H_exec.
+   inversion H_exec;subst.
+   inversion Htrans;subst.
+   simpl.
+   unfold funds.
+   simpl.
+   destruct_address_eq;try congruence.
+   lia.
+ Qed.
+
+  Lemma honest_call_PassHasBeenSetMsg_is_call_act_transition_correct_nopass:
+  forall (s:ChainState) cstate,
+      contract_state s caddr = Some cstate ->
+      transition_reachable miner contract caddr s0 s ->
+      cstate.(passHasBeenSet) = true ->
+      cstate.(hashPass) <> (sha3 honest_pass) ->
+      transition miner s (honest_call_PassHasBeenSetMsg cstate) = Err StratModel.default_error.
+  Proof.
+      intros * Hcs_s Htrc_s H_passB H_neq.
+      unfold transition.
+      unfold queue_isb_empty.
+      eapply transition_reachable_queue_is_empty in Htrc_s as Hqueue_s;eauto.
+      rewrite Hqueue_s.
+      rewrite honest_call_PassHasBeenSetMsg_is_call_act.
+      unfold evaluate_action.
+      rewrite get_valid_header_is_valid_header.
+      unfold honest_call_PassHasBeenSetMsg .
+      simpl.
+      destruct_address_eq;try congruence.
+      simpl.
+      assert (Hec_s:env_contracts s caddr = Some (contract:WeakContract)).
+      {
+        eapply transition_reachable_impl_reachable_through in Htrc_s.
+        eapply reachable_through_contract_deployed in Htrc_s;eauto.
+        decompose_is_init_state H_init.
+        eauto.
+        eauto.
+      }
+      eapply address_not_contract_negb in honest_eoa.
+      rewrite honest_eoa.
+      unfold send_or_call.
+      simpl.
+      assert( H_caddr_not_EOA : address_is_contract caddr = true).
+      {
+        eapply contract_addr_format in Hec_s;eauto.
+        eapply transition_reachable_impl_reachable in Htrc_s;eauto.  
+      }
+      assert(Hrc_s:reachable s).
+      {
+        eapply transition_reachable_impl_reachable in Htrc_s;eauto.
+      }
+      assert(Hbal:env_account_balances s caddr = cstate.(balance)).
+      {
+        eapply balance_on_chain_forall;eauto.
+        unfold outgoing_acts.
+        rewrite Hqueue_s.
+        simpl.
+        eauto.
+      }
+      destruct_address_eq;try congruence.
+      + assert ((0 >? miner_reward + env_account_balances s honest )%Z 
+                  = false).
+        {
+          unfold miner_reward.
+          eapply (account_balance_nonnegative s honest) in Hrc_s.
+          lia.
+        }
+        rewrite H.
+        rewrite Hec_s.
+        unfold contract_state in Hcs_s.
+        simpl in Hcs_s.
+        destruct (env_contract_states s caddr) eqn : Hecs_s;try congruence.
+        simpl.
+        rewrite Hcs_s.
+        simpl.
+        setoid_rewrite deserialize_serialize.
+        simpl.
+        cbn in *.
+        unfold receive.
+        destruct (hashPass cstate)%N eqn : HH.
+        - propify.  intuition.
+        - propify. 
+          unfold sha3 in H_neq.
+          destruct ((countable.encode honest_pass =? p)%positive) eqn :  h';try congruence .
+          propify.
+          eapply Pos.eqb_eq in h'.
+          rewrite <- h' in H_neq.
+          intuition.
+          setoid_rewrite h'.
+          simpl.
+          eauto.
+      
+      + assert ((0 >?  env_account_balances s honest )%Z 
+                  = false).
+        {
+          unfold miner_reward.
+          eapply (account_balance_nonnegative s honest) in Hrc_s.
+          lia.
+        }
+        rewrite H.
+        rewrite Hec_s.
+        unfold contract_state in Hcs_s.
+        simpl in Hcs_s.
+        destruct (env_contract_states s caddr) eqn : Hecs_s;try congruence.
+        simpl.
+        rewrite Hcs_s.
+        simpl.
+        setoid_rewrite deserialize_serialize.
+        simpl.
+        cbn in *.
+        unfold receive.
+        simpl.
+        unfold address_not_contract.
+        destruct (hashPass cstate)%N eqn : HH.
+        - propify.  intuition.
+        - propify. 
+          unfold sha3 in H_neq.
+          destruct ((countable.encode honest_pass =? p)%positive) eqn :  h';try congruence .
+          propify.
+          eapply Pos.eqb_eq in h'.
+          rewrite <- h' in H_neq.
+          intuition.
+          setoid_rewrite h'.
+          simpl.
+          eauto.
+      + assert ((0 >?  env_account_balances s honest )%Z 
+                  = false).
+        {
+          unfold miner_reward.
+          eapply (account_balance_nonnegative s honest) in Hrc_s.
+          lia.
+        }
+        rewrite H.
+        rewrite Hec_s.
+        unfold contract_state in Hcs_s.
+        simpl in Hcs_s.
+        destruct (env_contract_states s caddr) eqn : Hecs_s;try congruence.
+        simpl.
+        rewrite Hcs_s.
+        simpl.
+        setoid_rewrite deserialize_serialize.
+        simpl.
+        cbn in *.
+        unfold receive.
+        simpl.
+        unfold address_not_contract.
+        destruct (hashPass cstate)%N eqn : HH.
+        - propify.  intuition.
+        - propify. 
+          unfold sha3 in H_neq.
+          destruct ((countable.encode honest_pass =? p)%positive) eqn :  h';try congruence .
+          propify.
+          eapply Pos.eqb_eq in h'.
+          rewrite <- h' in H_neq.
+          intuition.
+          setoid_rewrite h'.
+          simpl.
+          eauto.
+  Qed.
+
+  Lemma honest_strat_correct_nopass:
+    forall (s s':ChainState) cstate a (tr : TransitionTrace miner s0 s) ,
+        contract_state s caddr = Some cstate ->
+        transition_reachable miner contract caddr s0 s ->
+        cstate.(passHasBeenSet) = true ->
+        cstate.(hashPass) <> (sha3 honest_pass) ->
+        In a (honest_strat s0 s tr) ->
+        transition miner s a = Ok s' ->
+        funds s' caddr >= funds s caddr.
+  Proof.
+    intros.
+    unfold honest_strat in *.
+    unfold get_contract_state in H3.
+    pose proof H as HT.
+    unfold contract_state in HT.
+    simpl in HT.
+    destruct (env_contract_states s caddr) eqn : cs;try congruence.
+    rewrite HT in H3.
+    destruct H3.
+    rewrite <- H3 in H4.
+    eapply honest_call_SetPass_is_call_act_state_correct in H4;eauto.
+    destruct H3.
+    rewrite <- H3 in H4.
+    eapply honest_call_GetGift_is_call_act_transition_correct_nopass in H;eauto.
+    congruence.
+    destruct H3.
+    eauto.
+    rewrite <- H3 in H4.
+    eapply honest_call_PassHasBeenSetMsg_is_call_act_transition_correct_nopass in H;eauto.
+    congruence.
+    destruct H3.
+  Qed.
+
+  Lemma attacker_call_SetPass_is_call_act_transition_correct:
+    forall (s:ChainState) cstate,
+        contract_state s caddr = Some cstate ->
+        transition_reachable miner contract caddr s0 s ->
+        cstate.(passHasBeenSet) = false ->
+        exists s',
+        transition miner s (attacker_call_SetPass cstate) = Ok s'.
+  Proof.
+    intros * Hcs_s Htrc_s H_passB  .
+    eexists.
+    unfold transition.
+    unfold queue_isb_empty.
+    eapply transition_reachable_queue_is_empty in Htrc_s as Hqueue_s;eauto.
+    rewrite Hqueue_s.
+    rewrite attacker_call_SetPass_is_call_act.
+    unfold evaluate_action.
+    rewrite get_valid_header_is_valid_header.
+    unfold attacker_call_SetPass .
+    simpl.
+    destruct_address_eq;try congruence.
+    simpl.
+    assert (Hec_s:env_contracts s caddr = Some (contract:WeakContract)).
+    {
+      eapply transition_reachable_impl_reachable_through in Htrc_s.
+      eapply reachable_through_contract_deployed in Htrc_s;eauto.
+      decompose_is_init_state H_init.
+      eauto.
+      eauto.
+    }
+    eapply address_not_contract_negb in attacker_eoa.
+    rewrite attacker_eoa.
+    unfold send_or_call.
+    simpl.
+    assert( H_caddr_not_EOA : address_is_contract caddr = true).
+    {
+      eapply contract_addr_format in Hec_s;eauto.
+      eapply transition_reachable_impl_reachable in Htrc_s;eauto.  
+    }
+    assert(Hrc_s:reachable s).
+    {
+      eapply transition_reachable_impl_reachable in Htrc_s;eauto.
+    }
+    assert(Hbal:env_account_balances s caddr = cstate.(balance)).
+    {
+      eapply balance_on_chain_forall;eauto.
+      unfold outgoing_acts.
+      rewrite Hqueue_s.
+      simpl.
+      eauto.
+    }
+    destruct_address_eq;try congruence.
+    + assert ((1 >? miner_reward + env_account_balances s attacker )%Z = false).
+      {
+        unfold miner_reward.
+        eapply (account_balance_nonnegative s attacker) in Hrc_s.
+        
+        lia.
+      }
+      rewrite H.
+      rewrite Hec_s.
+      unfold contract_state in Hcs_s.
+      simpl in Hcs_s.
+      destruct (env_contract_states s caddr) eqn : Hecs_s;try congruence.
+      simpl.
+      rewrite Hcs_s.
+      simpl.
+      setoid_rewrite deserialize_serialize.
+      simpl.
+      unfold setPass.
+      rewrite H_passB.
+      simpl.
+      eauto.
+      
+    + assert ((1 >? env_account_balances s attacker )%Z = false).
+    {
+      unfold miner_reward.
+      eapply (account_balance_nonnegative s attacker) in Hrc_s.
+      specialize (H_attack_bal_ge_1 s).
+      unfold funds in *.
+      lia.
+    }
+    rewrite H.
+    rewrite Hec_s.
+    unfold contract_state in Hcs_s.
+    simpl in Hcs_s.
+    destruct (env_contract_states s caddr) eqn : Hecs_s;try congruence.
+    simpl.
+    rewrite Hcs_s.
+    simpl.
+    setoid_rewrite deserialize_serialize.
+    simpl.
+    unfold setPass.
+    rewrite H_passB.
+    simpl.
+    eauto.
+    + assert ((1 >? env_account_balances s attacker )%Z 
+                = false).
+      {
+        unfold miner_reward.
+        eapply (account_balance_nonnegative s attacker) in Hrc_s.
+        specialize (H_attack_bal_ge_1 s).
+        unfold funds in *.
+        lia.
+      }
+      rewrite H.
+    rewrite Hec_s.
+    unfold contract_state in Hcs_s.
+    simpl in Hcs_s.
+    destruct (env_contract_states s caddr) eqn : Hecs_s;try congruence.
+    simpl.
+    rewrite Hcs_s.
+    simpl.
+    setoid_rewrite deserialize_serialize.
+    simpl.
+    unfold setPass.
+    rewrite H_passB.
+    simpl.
+    eauto.
+  Qed.
+
+  Lemma attacker_call_PassHasBeenSetMsg_is_call_act_transition_correct:
+    forall (s:ChainState) cstate,
+      contract_state s caddr = Some cstate ->
+      transition_reachable miner contract caddr s0 s ->
+      cstate.(passHasBeenSet) = false ->
+      cstate.(hashPass) = sha3 attacker_pass ->
+      exists s',
+      transition miner s (attacker_call_PassHasBeenSetMsg cstate) = Ok s'.
+  Proof.
+    intros * Hcs_s Htrc_s H_passB H_pass .
+    eexists.
+    unfold transition.
+    unfold queue_isb_empty.
+    eapply transition_reachable_queue_is_empty in Htrc_s as Hqueue_s;eauto.
+    rewrite Hqueue_s.
+    rewrite attacker_call_PassHasBeenSetMsg_is_call_act.
+    unfold evaluate_action.
+    rewrite get_valid_header_is_valid_header.
+    unfold attacker_call_PassHasBeenSetMsg .
+    simpl.
+    destruct_address_eq;try congruence.
+    simpl.
+    assert (Hec_s:env_contracts s caddr = Some (contract:WeakContract)).
+    {
+      eapply transition_reachable_impl_reachable_through in Htrc_s.
+      eapply reachable_through_contract_deployed in Htrc_s;eauto.
+      decompose_is_init_state H_init.
+      eauto.
+      eauto.
+    }
+    eapply address_not_contract_negb in attacker_eoa.
+    rewrite attacker_eoa.
+    unfold send_or_call.
+    simpl.
+    assert( H_caddr_not_EOA : address_is_contract caddr = true).
+    {
+      eapply contract_addr_format in Hec_s;eauto.
+      eapply transition_reachable_impl_reachable in Htrc_s;eauto.  
+    }
+    assert(Hrc_s:reachable s).
+    {
+      eapply transition_reachable_impl_reachable in Htrc_s;eauto.
+    }
+    assert(Hbal:env_account_balances s caddr = cstate.(balance)).
+    {
+      eapply balance_on_chain_forall;eauto.
+      unfold outgoing_acts.
+      rewrite Hqueue_s.
+      simpl.
+      eauto.
+    }
+    destruct_address_eq;try congruence.
+    + assert ((0 >? miner_reward + env_account_balances s attacker )%Z 
+                = false).
+      {
+        unfold miner_reward.
+        eapply (account_balance_nonnegative s attacker) in Hrc_s.
+        lia.
+      }
+      rewrite H.
+      rewrite Hec_s.
+      unfold contract_state in Hcs_s.
+      simpl in Hcs_s.
+      destruct (env_contract_states s caddr) eqn : Hecs_s;try congruence.
+      simpl.
+      rewrite Hcs_s.
+      simpl.
+      setoid_rewrite deserialize_serialize.
+      simpl.
+      cbn in *.
+      unfold receive.
+      simpl.
+      unfold address_not_contract.
+      rewrite H_pass.
+      destruct (hashPass cstate =? sha3 attacker_pass)%N eqn : N.
+      - propify. 
+        destruct (sha3 attacker_pass) eqn : h'; try congruence.
+        destruct ((countable.encode attacker_pass =? p)%positive) eqn : h''; try congruence.
+        ++ propify.
+           setoid_rewrite h''.
+           simpl.
+           eauto.
+        ++ eapply Pos.eqb_neq in h''.
+            unfold sha3 in h'.
+            eapply pos_inj in h'.
+            intuition.
+      - eapply N.eqb_neq in N.
+         rewrite H_pass in N.
+          intuition.
+      
+    + eapply address_not_contract_negb in H_miner.
+      rewrite e1 in *.
+      intuition.
+    + assert ((0 >?  env_account_balances s attacker )%Z 
+                = false).
+      {
+        unfold miner_reward.
+        eapply (account_balance_nonnegative s attacker) in Hrc_s.
+        specialize (H_honest_bal_ge_1 s).
+        unfold funds in *.
+        lia.
+      }
+      rewrite H.
+      rewrite Hec_s.
+      unfold contract_state in Hcs_s.
+      simpl in Hcs_s.
+      destruct (env_contract_states s caddr) eqn : Hecs_s;try congruence.
+      simpl.
+      rewrite Hcs_s.
+      simpl.
+      setoid_rewrite deserialize_serialize.
+      simpl.
+      cbn in *.
+      unfold receive.
+      simpl.
+      unfold address_not_contract.
+      rewrite H_pass.
+      destruct (hashPass cstate =? sha3 attacker_pass)%N eqn : N.
+      - propify. 
+        destruct (sha3 attacker_pass) eqn : h'; try congruence.
+        destruct ((countable.encode attacker_pass =? p)%positive) eqn : h''; try congruence.
+        ++ propify.
+           setoid_rewrite h''.
+           simpl.
+           eauto.
+        ++ eapply Pos.eqb_neq in h''.
+            unfold sha3 in h'.
+            eapply pos_inj in h'.
+            intuition.
+      - eapply N.eqb_neq in N.
+         rewrite H_pass in N.
+          intuition.
+  Qed.
+
+  Lemma attacker_call_SetPass_is_call_act_state_correct:
+   forall (s s':ChainState) cstate,
+      contract_state s caddr = Some cstate ->
+      transition_reachable miner contract caddr s0 s ->
+      cstate.(passHasBeenSet) = false ->
+      transition miner s (attacker_call_SetPass cstate) = Ok s' ->
+      exists cstate',
+        contract_state s' caddr = Some cstate' /\
+        cstate'.(hashPass) = sha3 attacker_pass /\
+        cstate'.(passHasBeenSet ) = false.
+  Proof.
+    intros * Hcs_s Htrc_s H_passB Htrans.
+    eapply transition_reachable_queue_is_empty in Htrc_s as Hqueue_s;eauto.
+    assert (Hact_call : is_call_act ((attacker_call_SetPass cstate)) = true).
+    {
+      unfold is_call_act.
+      unfold attacker_call_SetPass.
+      unfold build_call.
+      destruct_address_eq;eauto.
+    }
+    assert(ttrace_s_s : TransitionTrace miner s s) by eapply clnil.
+    assert(ttrace_s_s' : TransitionTrace miner s s').
+    {
+      econstructor;eauto.
+      eapply step_trans;eauto.
+
+    }
+    assert(Htrct_s_s' : reachable_via miner contract caddr s0 s s').
+    {
+      econstructor;eauto.
+    }
+    assert(Hrt : reachable_through s s').
+    {
+      eapply reachable_via_impl_reachable_through in Htrct_s_s';eauto.
+    }
+    assert(H_t: reachable s') by eauto.
+    destruct H_t as [trace].
+    assert (Hec_s : env_contracts s caddr = Some ((contract : WeakContract))).
+    {
+      pose proof H_init.
+      decompose_is_init_state H_init.
+      eapply reachable_through_contract_deployed in H_env_contracts.
+      eauto.
+      eapply transition_reachable_impl_reachable_through in Htrc_s;eauto.
+    }
+    assert (Hec_s' : env_contracts s' caddr = Some ((contract : WeakContract))).
+    {
+      pose proof H_init.
+      decompose_is_init_state H_init.
+      eapply reachable_through_contract_deployed in H_env_contracts.
+      eauto.
+      eapply transition_reachable_impl_reachable_through in Htrc_s;eauto.
+    }
+    eapply deployed_contract_state_typed in Hec_s';eauto.
+    destruct Hec_s' as [cstate_s' Hcs_s'].
+    exists cstate_s'.
+    split.
+    eauto.
+    unfold transition in Htrans.
+    unfold queue_isb_empty in Htrans.
+    rewrite Hqueue_s in Htrans.
+    rewrite Hact_call in Htrans.
+    destruct (evaluate_action true s (get_valid_header miner s)
+    [attacker_call_SetPass cstate ]) eqn : H_exec;try congruence.
+    unfold evaluate_action in H_exec.
+    rewrite get_valid_header_is_valid_header in H_exec.
+    destruct (find_origin_neq_from [attacker_call_SetPass cstate]) ; try congruence.
+    destruct (find_invalid_root_action [attacker_call_SetPass cstate]);try congruence.
+    set (mid_state := {|
+      chain_state_env := add_new_block_to_env (get_valid_header miner s) s;
+      chain_state_queue := [attacker_call_SetPass cstate]
+    |}) in H_exec.
+    simpl in *.
+    destruct(
+    send_or_call attacker attacker caddr 1
+      (Some (serialize (SetPass (sha3 attacker_pass))))
+      (add_new_block_to_env (get_valid_header miner s) s)) eqn : H_send_or_call_GetGift;try congruence.
+    unfold send_or_call in  H_send_or_call_GetGift.
+    simpl in H_send_or_call_GetGift.
+    eapply address_not_contract_negb in H_miner.
+    assert( H_caddr_not_EOA : address_is_contract caddr = true).
+    {
+      eapply contract_addr_format in Hec_s;eauto.
+      eapply transition_reachable_impl_reachable in Htrc_s;eauto.  
+    }
+    destruct_address_eq;simpl in *;try congruence.
+    
+    (* 
+      e: sender cstate = miner
+      n: caddr <> sender cstate
+      e0: caddr = caddr
+      n0: caddr <> miner 
+    *)
+
+    destruct(1 >? miner_reward + env_account_balances s attacker)%Z;try congruence.
+    rewrite Hec_s in H_send_or_call_GetGift.
+    assert(Hcstate_s_t0:contract_state s caddr = Some cstate) by eauto.
+    unfold contract_state in Hcstate_s_t0.
+    simpl in Hcstate_s_t0.
+    destruct (env_contract_states s caddr) eqn : Hcstate_s_t0';try congruence.
+    destruct (weak_error_to_error_receive
+    (wc_receive contract
+       (s <| chain_height := S (chain_height s) |> <|
+        current_slot := (current_slot s + 1)%nat |> <|
+        finalized_height := finalized_height s |>)
+       {|
+         ctx_origin := attacker;
+         ctx_from := attacker;
+         ctx_contract_address := caddr;
+         ctx_contract_balance :=
+           1 + env_account_balances s caddr;
+         ctx_amount := 1
+       |} s1
+       (Some (serialize (SetPass (sha3 attacker_pass)))))) eqn : H_wc_receive_s1;try congruence.
+    unfold weak_error_to_error_receive in H_wc_receive_s1.
+    unfold bind_error in H_wc_receive_s1.
+    destruct (wc_receive contract
+    (s <| chain_height := S (chain_height s) |> <| current_slot
+     := (current_slot s + 1)%nat |> <| finalized_height :=
+     finalized_height s |>)
+    {|
+      ctx_origin := attacker;
+      ctx_from := attacker;
+      ctx_contract_address := caddr;
+      ctx_contract_balance := 1 + env_account_balances s caddr;
+      ctx_amount := 1
+    |} s1 (Some (serialize (SetPass (sha3 attacker_pass)))))
+      eqn : H_wc_receive_s1';try congruence.
+    
+    set (cchain := s <| chain_height := S (chain_height s) |> <| current_slot :=
+    (current_slot s + 1)%nat |> <| finalized_height :=
+    finalized_height s |>) in H_wc_receive_s1'.
+    set (cctx := {|
+    ctx_origin := user1;
+    ctx_from := user1;
+    ctx_contract_address := caddr;
+    ctx_contract_balance := 0 + env_account_balances s caddr;
+    ctx_amount := 0
+    |}) in H_wc_receive_s1'.
+    
+    destruct t2 as [new_state new_acts].
+
+    destruct (wc_receive_strong ltac:(try eassumption))
+    as (prev_state_strong & msg_strong & resp_state_strong &
+      deser_state & deser_msg & <- & receive).
+
+    simpl in deser_msg.
+    destruct (msg_strong) eqn : H_msg;try congruence.
+    rewrite deserialize_serialize in deser_msg.
+    rewrite <- deser_msg in receive.
+    rewrite deser_state in Hcstate_s_t0.
+    simpl in receive.
+    rename receive into receive_some.
+    unfold receive in receive_some.
+    reduce_setPass.
+    (* 111 *)
+    inversion receive_some.
+    subst.
+    inversion H_wc_receive_s1;subst.
+    inversion H_send_or_call_GetGift;subst.
+    simpl in H_exec.
+    inversion H_exec;subst.
+    inversion Htrans;subst.
+    inversion H_send_or_call_GetGift;subst.
+    inversion Hcs_s';subst.
+    unfold contract_state in H0.
+    simpl in H0.
+    destruct_address_eq;eauto.
+    setoid_rewrite deserialize_serialize in H0.
+    inversion H0.
+    inversion Hcstate_s_t0 ;    subst.
+    intuition.
+    destruct_address_eq;try congruence.
+
+    simpl in *.
+    inversion Hcstate_s_t0.
+    rewrite H0 in EsetPass.
+    rewrite H_passB in EsetPass.
+    simpl in EsetPass.
+    unfold one_ether in EsetPass.
+    intuition.
+
+    (* n: attacker <> miner
+      e: caddr = attacker
+      e0: caddr = caddr
+      n0: caddr <> miner *)
+
+    eapply address_not_contract_negb in attacker_eoa.
+    rewrite e in *.
+    intuition.
+
+    (* 
+      n: attacker <> miner
+    n0: caddr <> attacker
+    e: caddr = caddr
+    n1: caddr <> miner
+    
+    *)
+    destruct(1 >?  env_account_balances s attacker)%Z;try congruence.
+    rewrite Hec_s in H_send_or_call_GetGift.
+    assert(Hcstate_s_t0:contract_state s caddr = Some cstate) by eauto.
+    unfold contract_state in Hcstate_s_t0.
+    simpl in Hcstate_s_t0.
+    destruct (env_contract_states s caddr) eqn : Hcstate_s_t0';try congruence.
+    destruct (weak_error_to_error_receive
+    (wc_receive contract
+       (s <| chain_height := S (chain_height s) |> <|
+        current_slot := (current_slot s + 1)%nat |> <|
+        finalized_height := finalized_height s |>)
+       {|
+         ctx_origin := attacker;
+         ctx_from := attacker;
+         ctx_contract_address := caddr;
+         ctx_contract_balance :=
+           1 + env_account_balances s caddr;
+         ctx_amount := 1
+       |} s1
+       (Some (serialize (SetPass (sha3 attacker_pass)))))) eqn : H_wc_receive_s1;try congruence.
+    unfold weak_error_to_error_receive in H_wc_receive_s1.
+    unfold bind_error in H_wc_receive_s1.
+    destruct (wc_receive contract
+    (s <| chain_height := S (chain_height s) |> <| current_slot
+     := (current_slot s + 1)%nat |> <| finalized_height :=
+     finalized_height s |>)
+    {|
+      ctx_origin := attacker;
+      ctx_from := attacker;
+      ctx_contract_address := caddr;
+      ctx_contract_balance := 1 + env_account_balances s caddr;
+      ctx_amount := 1
+    |} s1 (Some (serialize (SetPass (sha3 attacker_pass)))))
+      eqn : H_wc_receive_s1';try congruence.
+    
+    set (cchain := s <| chain_height := S (chain_height s) |> <| current_slot :=
+    (current_slot s + 1)%nat |> <| finalized_height :=
+    finalized_height s |>) in H_wc_receive_s1'.
+    set (cctx := {|
+    ctx_origin := user1;
+    ctx_from := user1;
+    ctx_contract_address := caddr;
+    ctx_contract_balance := 0 + env_account_balances s caddr;
+    ctx_amount := 0
+    |}) in H_wc_receive_s1'.
+    
+    destruct t2 as [new_state new_acts].
+
+    destruct (wc_receive_strong ltac:(try eassumption))
+    as (prev_state_strong & msg_strong & resp_state_strong &
+      deser_state & deser_msg & <- & receive).
+
+    simpl in deser_msg.
+    destruct (msg_strong) eqn : H_msg;try congruence.
+    rewrite deserialize_serialize in deser_msg.
+    rewrite <- deser_msg in receive.
+    rewrite deser_state in Hcstate_s_t0.
+    simpl in receive.
+    rename receive into receive_some.
+    unfold receive in receive_some.
+    reduce_setPass.
+    (* 111 *)
+    inversion receive_some.
+    subst.
+    inversion H_wc_receive_s1;subst.
+    inversion H_send_or_call_GetGift;subst.
+    simpl in H_exec.
+    inversion H_exec;subst.
+    inversion Htrans;subst.
+    inversion H_send_or_call_GetGift;subst.
+    inversion Hcs_s';subst.
+    unfold contract_state in H0.
+    simpl in H0.
+    destruct_address_eq;eauto.
+    setoid_rewrite deserialize_serialize in H0.
+    inversion H0.
+    inversion Hcstate_s_t0 ;    subst.
+    intuition.
+    destruct_address_eq;try congruence.
+    simpl in *.
+    inversion Hcstate_s_t0.
+    rewrite H0 in EsetPass.
+    rewrite H_passB in EsetPass.
+    simpl in EsetPass.
+    unfold one_ether in EsetPass.
+    intuition.
+  Qed.
+
+  Lemma attacker_call_SetPass_is_call_act_state_correct_funds:
+    forall (s s':ChainState) cstate,
+     contract_state s caddr = Some cstate ->
+     transition_reachable miner contract caddr s0 s ->
+     cstate.(passHasBeenSet) = false ->
+     transition miner s (attacker_call_SetPass cstate) = Ok s' ->
+     funds s' caddr > 0.
+  Proof.
+    intros * Hcs_s Htrc_s H_passB Htrans.
+    eapply transition_reachable_queue_is_empty in Htrc_s as Hqueue_s;eauto.
+    assert (Hact_call : is_call_act ((attacker_call_SetPass cstate)) = true).
+    {
+      unfold is_call_act.
+      unfold attacker_call_SetPass.
+      unfold build_call.
+      destruct_address_eq;eauto.
+    }
+    assert(ttrace_s_s : TransitionTrace miner s s) by eapply clnil.
+    assert(ttrace_s_s' : TransitionTrace miner s s').
+    {
+      econstructor;eauto.
+      eapply step_trans;eauto.
+
+    }
+    assert(Htrct_s_s' : reachable_via miner contract caddr s0 s s').
+    {
+      econstructor;eauto.
+    }
+    assert(Hrt : reachable_through s s').
+    {
+      eapply reachable_via_impl_reachable_through in Htrct_s_s';eauto.
+    }
+    assert(H_t: reachable s') by eauto.
+    destruct H_t as [trace].
+    assert (Hec_s : env_contracts s caddr = Some ((contract : WeakContract))).
+    {
+      pose proof H_init.
+      decompose_is_init_state H_init.
+      eapply reachable_through_contract_deployed in H_env_contracts.
+      eauto.
+      eapply transition_reachable_impl_reachable_through in Htrc_s;eauto.
+    }
+    assert (Hec_s' : env_contracts s' caddr = Some ((contract : WeakContract))).
+    {
+      pose proof H_init.
+      decompose_is_init_state H_init.
+      eapply reachable_through_contract_deployed in H_env_contracts.
+      eauto.
+      eapply transition_reachable_impl_reachable_through in Htrc_s;eauto.
+    }
+    eapply deployed_contract_state_typed in Hec_s';eauto.
+    
+    unfold transition in Htrans.
+    unfold queue_isb_empty in Htrans.
+    rewrite Hqueue_s in Htrans.
+    rewrite Hact_call in Htrans.
+    destruct (evaluate_action true s (get_valid_header miner s)
+    [attacker_call_SetPass cstate ]) eqn : H_exec;try congruence.
+    unfold evaluate_action in H_exec.
+    rewrite get_valid_header_is_valid_header in H_exec.
+    destruct (find_origin_neq_from [attacker_call_SetPass cstate]) ; try congruence.
+    destruct (find_invalid_root_action [attacker_call_SetPass cstate]);try congruence.
+    set (mid_state := {|
+      chain_state_env := add_new_block_to_env (get_valid_header miner s) s;
+      chain_state_queue := [attacker_call_SetPass cstate]
+    |}) in H_exec.
+    simpl in *.
+    destruct(
+    send_or_call attacker attacker caddr 1
+      (Some (serialize (SetPass (sha3 attacker_pass))))
+      (add_new_block_to_env (get_valid_header miner s) s)) eqn : H_send_or_call_GetGift;try congruence.
+    unfold send_or_call in  H_send_or_call_GetGift.
+    simpl in H_send_or_call_GetGift.
+    eapply address_not_contract_negb in H_miner.
+    assert( H_caddr_not_EOA : address_is_contract caddr = true).
+    {
+      eapply contract_addr_format in Hec_s;eauto.
+      eapply transition_reachable_impl_reachable in Htrc_s;eauto.  
+    }
+    destruct_address_eq;simpl in *;try congruence.
+    
+    (* 
+      e: sender cstate = miner
+      n: caddr <> sender cstate
+      e0: caddr = caddr
+      n0: caddr <> miner 
+    *)
+
+    destruct(1 >? miner_reward + env_account_balances s attacker)%Z;try congruence.
+    rewrite Hec_s in H_send_or_call_GetGift.
+    assert(Hcstate_s_t0:contract_state s caddr = Some cstate) by eauto.
+    unfold contract_state in Hcstate_s_t0.
+    simpl in Hcstate_s_t0.
+    destruct (env_contract_states s caddr) eqn : Hcstate_s_t0';try congruence.
+    destruct (weak_error_to_error_receive
+    (wc_receive contract
+       (s <| chain_height := S (chain_height s) |> <|
+        current_slot := (current_slot s + 1)%nat |> <|
+        finalized_height := finalized_height s |>)
+       {|
+         ctx_origin := attacker;
+         ctx_from := attacker;
+         ctx_contract_address := caddr;
+         ctx_contract_balance :=
+           1 + env_account_balances s caddr;
+         ctx_amount := 1
+       |} s1
+       (Some (serialize (SetPass (sha3 attacker_pass)))))) eqn : H_wc_receive_s1;try congruence.
+    unfold weak_error_to_error_receive in H_wc_receive_s1.
+    unfold bind_error in H_wc_receive_s1.
+    destruct (wc_receive contract
+    (s <| chain_height := S (chain_height s) |> <| current_slot
+     := (current_slot s + 1)%nat |> <| finalized_height :=
+     finalized_height s |>)
+    {|
+      ctx_origin := attacker;
+      ctx_from := attacker;
+      ctx_contract_address := caddr;
+      ctx_contract_balance := 1 + env_account_balances s caddr;
+      ctx_amount := 1
+    |} s1 (Some (serialize (SetPass (sha3 attacker_pass)))))
+      eqn : H_wc_receive_s1';try congruence.
+    
+    set (cchain := s <| chain_height := S (chain_height s) |> <| current_slot :=
+    (current_slot s + 1)%nat |> <| finalized_height :=
+    finalized_height s |>) in H_wc_receive_s1'.
+    set (cctx := {|
+    ctx_origin := user1;
+    ctx_from := user1;
+    ctx_contract_address := caddr;
+    ctx_contract_balance := 0 + env_account_balances s caddr;
+    ctx_amount := 0
+    |}) in H_wc_receive_s1'.
+    
+    destruct t2 as [new_state new_acts].
+
+    destruct (wc_receive_strong ltac:(try eassumption))
+    as (prev_state_strong & msg_strong & resp_state_strong &
+      deser_state & deser_msg & <- & receive).
+
+    simpl in deser_msg.
+    destruct (msg_strong) eqn : H_msg;try congruence.
+    rewrite deserialize_serialize in deser_msg.
+    rewrite <- deser_msg in receive.
+    rewrite deser_state in Hcstate_s_t0.
+    simpl in receive.
+    rename receive into receive_some.
+    unfold receive in receive_some.
+    reduce_setPass.
+    (* 111 *)
+    inversion receive_some.
+    subst.
+    inversion H_wc_receive_s1;subst.
+    inversion H_send_or_call_GetGift;subst.
+    simpl in H_exec.
+    inversion H_exec;subst.
+    inversion Htrans;subst.
+    inversion H_send_or_call_GetGift;subst.
+    eapply transition_reachable_impl_reachable in Htrc_s as Hreac.
+    eapply (reachable_funds_nonnegative s caddr) in Hreac.
+    unfold funds in *.
+    simpl.
+    destruct_address_eq;try congruence.
+    lia.
+    eauto.
+
+
+    simpl in *.
+    inversion Hcstate_s_t0.
+    rewrite H0 in EsetPass.
+    rewrite H_passB in EsetPass.
+    simpl in EsetPass.
+    unfold one_ether in EsetPass.
+    intuition.
+
+    (* n: attacker <> miner
+      e: caddr = attacker
+      e0: caddr = caddr
+      n0: caddr <> miner *)
+
+    eapply address_not_contract_negb in attacker_eoa.
+    rewrite e in *.
+    intuition.
+
+    (* 
+      n: attacker <> miner
+    n0: caddr <> attacker
+    e: caddr = caddr
+    n1: caddr <> miner
+    
+    *)
+    destruct(1 >?  env_account_balances s attacker)%Z;try congruence.
+    rewrite Hec_s in H_send_or_call_GetGift.
+    assert(Hcstate_s_t0:contract_state s caddr = Some cstate) by eauto.
+    unfold contract_state in Hcstate_s_t0.
+    simpl in Hcstate_s_t0.
+    destruct (env_contract_states s caddr) eqn : Hcstate_s_t0';try congruence.
+    destruct (weak_error_to_error_receive
+    (wc_receive contract
+       (s <| chain_height := S (chain_height s) |> <|
+        current_slot := (current_slot s + 1)%nat |> <|
+        finalized_height := finalized_height s |>)
+       {|
+         ctx_origin := attacker;
+         ctx_from := attacker;
+         ctx_contract_address := caddr;
+         ctx_contract_balance :=
+           1 + env_account_balances s caddr;
+         ctx_amount := 1
+       |} s1
+       (Some (serialize (SetPass (sha3 attacker_pass)))))) eqn : H_wc_receive_s1;try congruence.
+    unfold weak_error_to_error_receive in H_wc_receive_s1.
+    unfold bind_error in H_wc_receive_s1.
+    destruct (wc_receive contract
+    (s <| chain_height := S (chain_height s) |> <| current_slot
+     := (current_slot s + 1)%nat |> <| finalized_height :=
+     finalized_height s |>)
+    {|
+      ctx_origin := attacker;
+      ctx_from := attacker;
+      ctx_contract_address := caddr;
+      ctx_contract_balance := 1 + env_account_balances s caddr;
+      ctx_amount := 1
+    |} s1 (Some (serialize (SetPass (sha3 attacker_pass)))))
+      eqn : H_wc_receive_s1';try congruence.
+    
+    set (cchain := s <| chain_height := S (chain_height s) |> <| current_slot :=
+    (current_slot s + 1)%nat |> <| finalized_height :=
+    finalized_height s |>) in H_wc_receive_s1'.
+    set (cctx := {|
+    ctx_origin := user1;
+    ctx_from := user1;
+    ctx_contract_address := caddr;
+    ctx_contract_balance := 0 + env_account_balances s caddr;
+    ctx_amount := 0
+    |}) in H_wc_receive_s1'.
+    
+    destruct t2 as [new_state new_acts].
+
+    destruct (wc_receive_strong ltac:(try eassumption))
+    as (prev_state_strong & msg_strong & resp_state_strong &
+      deser_state & deser_msg & <- & receive).
+
+    simpl in deser_msg.
+    destruct (msg_strong) eqn : H_msg;try congruence.
+    rewrite deserialize_serialize in deser_msg.
+    rewrite <- deser_msg in receive.
+    rewrite deser_state in Hcstate_s_t0.
+    simpl in receive.
+    rename receive into receive_some.
+    unfold receive in receive_some.
+    reduce_setPass.
+    (* 111 *)
+    inversion receive_some.
+    subst.
+    inversion H_wc_receive_s1;subst.
+    inversion H_send_or_call_GetGift;subst.
+    simpl in H_exec.
+    inversion H_exec;subst.
+    inversion Htrans;subst.
+    inversion H_send_or_call_GetGift;subst.
+    eapply transition_reachable_impl_reachable in Htrc_s as Hreac.
+    eapply (reachable_funds_nonnegative s caddr) in Hreac.
+    unfold funds in *.
+    simpl.
+    destruct_address_eq;try congruence.
+    lia.
+    eauto.
+    simpl in *.
+    inversion Hcstate_s_t0.
+    rewrite H0 in EsetPass.
+    rewrite H_passB in EsetPass.
+    simpl in EsetPass.
+    unfold one_ether in EsetPass.
+    intuition.
+  Qed.
+
+  Lemma attacker_call_PassHasBeenSetMsg_is_call_act_state_correct_funds:
+  forall (s s':ChainState) cstate,
+      contract_state s caddr = Some cstate ->
+      transition_reachable miner contract caddr s0 s ->
+      cstate.(passHasBeenSet) = false ->
+      cstate.(hashPass) = sha3 attacker_pass ->
+      transition miner s (attacker_call_PassHasBeenSetMsg cstate) = Ok s' ->
+      funds s' caddr = funds s caddr.
+  Proof.
+    intros * Hcs_s Htrc_s H_passB H_pass Htrans.
+    eapply transition_reachable_queue_is_empty in Htrc_s as Hqueue_s;eauto.
+    assert (Hact_call : is_call_act ((attacker_call_PassHasBeenSetMsg cstate)) = true).
+    {
+      unfold is_call_act.
+      unfold attacker_call_PassHasBeenSetMsg.
+      unfold build_call.
+      destruct_address_eq;eauto.
+    }
+    assert(ttrace_s_s : TransitionTrace miner s s) by eapply clnil.
+    assert(ttrace_s_s' : TransitionTrace miner s s').
+    {
+      econstructor;eauto.
+      eapply step_trans;eauto.
+    }
+    assert(Htrct_s_s' : reachable_via miner contract caddr s0 s s').
+    {
+      econstructor;eauto.
+    }
+    assert(Hrt : reachable_through s s').
+    {
+      eapply reachable_via_impl_reachable_through in Htrct_s_s';eauto.
+    }
+    assert(H_t: reachable s') by eauto.
+    destruct H_t as [trace].
+    assert (Hec_s : env_contracts s caddr = Some ((contract : WeakContract))).
+    {
+      pose proof H_init.
+      decompose_is_init_state H_init.
+      eapply reachable_through_contract_deployed in H_env_contracts.
+      eauto.
+      eapply transition_reachable_impl_reachable_through in Htrc_s;eauto.
+    }
+    assert (Hec_s' : env_contracts s' caddr = Some ((contract : WeakContract))).
+    {
+      pose proof H_init.
+      decompose_is_init_state H_init.
+      eapply reachable_through_contract_deployed in H_env_contracts.
+      eauto.
+      eapply transition_reachable_impl_reachable_through in Htrc_s;eauto.
+    }
+    eapply deployed_contract_state_typed in Hec_s';eauto.
+    destruct Hec_s' as [cstate_s' Hcs_s'].
+    
+    eauto.
+    unfold transition in Htrans.
+    unfold queue_isb_empty in Htrans.
+    rewrite Hqueue_s in Htrans.
+    rewrite Hact_call in Htrans.
+    destruct (evaluate_action true s (get_valid_header miner s)
+    [attacker_call_PassHasBeenSetMsg cstate ]) eqn : H_exec;try congruence.
+    unfold evaluate_action in H_exec.
+    rewrite get_valid_header_is_valid_header in H_exec.
+    destruct (find_origin_neq_from [attacker_call_PassHasBeenSetMsg cstate]) ; try congruence.
+    destruct (find_invalid_root_action [attacker_call_PassHasBeenSetMsg cstate]);try congruence.
+    set (mid_state := {|
+      chain_state_env := add_new_block_to_env (get_valid_header miner s) s;
+      chain_state_queue := [attacker_call_PassHasBeenSetMsg cstate]
+    |}) in H_exec.
+    simpl in *.
+    destruct(
+      send_or_call attacker attacker caddr 0
+      (Some (serialize (PassHasBeenSetMsg (sha3 attacker_pass))))
+      (add_new_block_to_env (get_valid_header miner s) s)) eqn : H_send_or_call_GetGift;try congruence.
+    unfold send_or_call in  H_send_or_call_GetGift.
+    simpl in H_send_or_call_GetGift.
+    eapply address_not_contract_negb in H_miner.
+    assert( H_caddr_not_EOA : address_is_contract caddr = true).
+    {
+      eapply contract_addr_format in Hec_s;eauto.
+      eapply transition_reachable_impl_reachable in Htrc_s;eauto.  
+    }
+    destruct_address_eq;simpl in *;try congruence.
+    
+    (* 
+      e: sender cstate = miner
+      n: caddr <> sender cstate
+      e0: caddr = caddr
+      n0: caddr <> miner 
+    *)
+
+    destruct(0 >? miner_reward + env_account_balances s attacker)%Z;try congruence.
+    rewrite Hec_s in H_send_or_call_GetGift.
+    assert(Hcstate_s_t0:contract_state s caddr = Some cstate) by eauto.
+    unfold contract_state in Hcstate_s_t0.
+    simpl in Hcstate_s_t0.
+    destruct (env_contract_states s caddr) eqn : Hcstate_s_t0';try congruence.
+    destruct (weak_error_to_error_receive
+    (wc_receive contract
+       (s <| chain_height := S (chain_height s) |> <|
+        current_slot := (current_slot s + 1)%nat |> <|
+        finalized_height := finalized_height s |>)
+       {|
+         ctx_origin := attacker;
+         ctx_from := attacker;
+         ctx_contract_address := caddr;
+         ctx_contract_balance :=
+           0 + env_account_balances s caddr;
+         ctx_amount := 0
+       |} s1
+       (Some
+          (serialize
+             (PassHasBeenSetMsg (sha3 attacker_pass)))))) eqn : H_wc_receive_s1;try congruence.
+    unfold weak_error_to_error_receive in H_wc_receive_s1.
+    unfold bind_error in H_wc_receive_s1.
+    destruct (wc_receive contract
+    (s <| chain_height := S (chain_height s) |> <| current_slot
+     := (current_slot s + 1)%nat |> <| finalized_height :=
+     finalized_height s |>)
+    {|
+      ctx_origin := attacker;
+      ctx_from := attacker;
+      ctx_contract_address := caddr;
+      ctx_contract_balance := 0 + env_account_balances s caddr;
+      ctx_amount := 0
+    |} s1
+    (Some (serialize (PassHasBeenSetMsg (sha3 attacker_pass)))))
+      eqn : H_wc_receive_s1';try congruence.
+    
+    set (cchain := s <| chain_height := S (chain_height s) |> <| current_slot :=
+    (current_slot s + 1)%nat |> <| finalized_height :=
+    finalized_height s |>) in H_wc_receive_s1'.
+    set (cctx := {|
+    ctx_origin := user1;
+    ctx_from := user1;
+    ctx_contract_address := caddr;
+    ctx_contract_balance := 0 + env_account_balances s caddr;
+    ctx_amount := 0
+    |}) in H_wc_receive_s1'.
+    
+    destruct t2 as [new_state new_acts].
+
+    destruct (wc_receive_strong ltac:(try eassumption))
+    as (prev_state_strong & msg_strong & resp_state_strong &
+      deser_state & deser_msg & <- & receive).
+
+    simpl in deser_msg.
+    destruct (msg_strong) eqn : H_msg;try congruence.
+    rewrite deserialize_serialize in deser_msg.
+    rewrite <- deser_msg in receive.
+    rewrite deser_state in Hcstate_s_t0.
+    simpl in receive.
+    rename receive into receive_some.
+    unfold receive in receive_some.
+    reduce_passHasBeenSet_fn.
+    (* 111 *)
+    inversion receive_some.
+    subst.
+    inversion H_wc_receive_s1;subst.
+    inversion H_send_or_call_GetGift;subst.
+    simpl in H_exec.
+    inversion H_exec;subst.
+    inversion Htrans;subst.
+    inversion H_send_or_call_GetGift;subst.
+    inversion Hcs_s';subst.
+    unfold contract_state in H0.
+    simpl in H0.
+    destruct_address_eq;eauto.
+    setoid_rewrite deserialize_serialize in H0.
+    inversion H0.
+    simpl.
+    inversion Hcstate_s_t0.
+    unfold funds.
+    simpl.
+    destruct_address_eq;try congruence.
+    eauto.
+    unfold funds.
+    simpl.
+    destruct_address_eq;try congruence.
+    eauto.
+    (* n: attacker <> miner
+      e: caddr = attacker
+      e0: caddr = caddr
+      n0: caddr <> miner *)
+    eapply address_not_contract_negb in attacker_eoa.
+    rewrite e in *.
+    intuition.
+    (* 
+      n: attacker <> miner
+    n0: caddr <> attacker
+    e: caddr = caddr
+    n1: caddr <> miner
+    
+    *)
+    destruct(0 >?  env_account_balances s attacker)%Z;try congruence.
+    rewrite Hec_s in H_send_or_call_GetGift.
+    assert(Hcstate_s_t0:contract_state s caddr = Some cstate) by eauto.
+    unfold contract_state in Hcstate_s_t0.
+    simpl in Hcstate_s_t0.
+    destruct (env_contract_states s caddr) eqn : Hcstate_s_t0';try congruence.
+    destruct (weak_error_to_error_receive
+    (wc_receive contract
+       (s <| chain_height := S (chain_height s) |> <|
+        current_slot := (current_slot s + 1)%nat |> <|
+        finalized_height := finalized_height s |>)
+       {|
+         ctx_origin := attacker;
+         ctx_from := attacker;
+         ctx_contract_address := caddr;
+         ctx_contract_balance :=
+           0 + env_account_balances s caddr;
+         ctx_amount := 0
+       |} s1
+       (Some
+          (serialize
+             (PassHasBeenSetMsg (sha3 attacker_pass)))))) eqn : H_wc_receive_s1;try congruence.
+    unfold weak_error_to_error_receive in H_wc_receive_s1.
+    unfold bind_error in H_wc_receive_s1.
+    destruct (wc_receive contract
+    (s <| chain_height := S (chain_height s) |> <| current_slot
+     := (current_slot s + 1)%nat |> <| finalized_height :=
+     finalized_height s |>)
+    {|
+      ctx_origin := attacker;
+      ctx_from := attacker;
+      ctx_contract_address := caddr;
+      ctx_contract_balance := 0 + env_account_balances s caddr;
+      ctx_amount := 0
+    |} s1
+    (Some (serialize (PassHasBeenSetMsg (sha3 attacker_pass)))))
+      eqn : H_wc_receive_s1';try congruence.
+    
+    set (cchain := s <| chain_height := S (chain_height s) |> <| current_slot :=
+    (current_slot s + 1)%nat |> <| finalized_height :=
+    finalized_height s |>) in H_wc_receive_s1'.
+    set (cctx := {|
+    ctx_origin := user1;
+    ctx_from := user1;
+    ctx_contract_address := caddr;
+    ctx_contract_balance := 0 + env_account_balances s caddr;
+    ctx_amount := 0
+    |}) in H_wc_receive_s1'.
+    
+    destruct t2 as [new_state new_acts].
+
+    destruct (wc_receive_strong ltac:(try eassumption))
+    as (prev_state_strong & msg_strong & resp_state_strong &
+      deser_state & deser_msg & <- & receive).
+
+    simpl in deser_msg.
+    destruct (msg_strong) eqn : H_msg;try congruence.
+    rewrite deserialize_serialize in deser_msg.
+    rewrite <- deser_msg in receive.
+    rewrite deser_state in Hcstate_s_t0.
+    simpl in receive.
+    rename receive into receive_some.
+    unfold receive in receive_some.
+    reduce_passHasBeenSet_fn.
+    (* 111 *)
+    inversion receive_some.
+    subst.
+    inversion H_wc_receive_s1;subst.
+    inversion H_send_or_call_GetGift;subst.
+    simpl in H_exec.
+    inversion H_exec;subst.
+    inversion Htrans;subst.
+    inversion H_send_or_call_GetGift;subst.
+    inversion Hcs_s';subst.
+    unfold contract_state in H0.
+    simpl in H0.
+    destruct_address_eq;eauto.
+    setoid_rewrite deserialize_serialize in H0.
+    inversion H0.
+    simpl.
+    inversion Hcstate_s_t0.
+    unfold funds.
+    simpl.
+    destruct_address_eq;try congruence.
+    eauto.
+    unfold funds.
+    simpl.
+    destruct_address_eq;try congruence.
+  Qed.
+
+  Lemma attacker_call_PassHasBeenSetMsg_is_call_act_state_correct:
+  forall (s s':ChainState) cstate,
+      contract_state s caddr = Some cstate ->
+      transition_reachable miner contract caddr s0 s ->
+      cstate.(passHasBeenSet) = false ->
+      cstate.(hashPass) = sha3 attacker_pass ->
+      transition miner s (attacker_call_PassHasBeenSetMsg cstate) = Ok s' ->
+      exists cstate',
+        contract_state s' caddr = Some cstate' /\
+        cstate'.(hashPass) = sha3 attacker_pass /\
+        cstate'.(passHasBeenSet) = true.
+  Proof.
+    intros * Hcs_s Htrc_s H_passB H_pass Htrans.
+    eapply transition_reachable_queue_is_empty in Htrc_s as Hqueue_s;eauto.
+    assert (Hact_call : is_call_act ((attacker_call_PassHasBeenSetMsg cstate)) = true).
+    {
+      unfold is_call_act.
+      unfold attacker_call_PassHasBeenSetMsg.
+      unfold build_call.
+      destruct_address_eq;eauto.
+    }
+    assert(ttrace_s_s : TransitionTrace miner s s) by eapply clnil.
+    assert(ttrace_s_s' : TransitionTrace miner s s').
+    {
+      econstructor;eauto.
+      eapply step_trans;eauto.
+    }
+    assert(Htrct_s_s' : reachable_via miner contract caddr s0 s s').
+    {
+      econstructor;eauto.
+    }
+    assert(Hrt : reachable_through s s').
+    {
+      eapply reachable_via_impl_reachable_through in Htrct_s_s';eauto.
+    }
+    assert(H_t: reachable s') by eauto.
+    destruct H_t as [trace].
+    assert (Hec_s : env_contracts s caddr = Some ((contract : WeakContract))).
+    {
+      pose proof H_init.
+      decompose_is_init_state H_init.
+      eapply reachable_through_contract_deployed in H_env_contracts.
+      eauto.
+      eapply transition_reachable_impl_reachable_through in Htrc_s;eauto.
+    }
+    assert (Hec_s' : env_contracts s' caddr = Some ((contract : WeakContract))).
+    {
+      pose proof H_init.
+      decompose_is_init_state H_init.
+      eapply reachable_through_contract_deployed in H_env_contracts.
+      eauto.
+      eapply transition_reachable_impl_reachable_through in Htrc_s;eauto.
+    }
+    eapply deployed_contract_state_typed in Hec_s';eauto.
+    destruct Hec_s' as [cstate_s' Hcs_s'].
+    exists cstate_s'.
+    split.
+    eauto.
+    unfold transition in Htrans.
+    unfold queue_isb_empty in Htrans.
+    rewrite Hqueue_s in Htrans.
+    rewrite Hact_call in Htrans.
+    destruct (evaluate_action true s (get_valid_header miner s)
+    [attacker_call_PassHasBeenSetMsg cstate ]) eqn : H_exec;try congruence.
+    unfold evaluate_action in H_exec.
+    rewrite get_valid_header_is_valid_header in H_exec.
+    destruct (find_origin_neq_from [attacker_call_PassHasBeenSetMsg cstate]) ; try congruence.
+    destruct (find_invalid_root_action [attacker_call_PassHasBeenSetMsg cstate]);try congruence.
+    set (mid_state := {|
+      chain_state_env := add_new_block_to_env (get_valid_header miner s) s;
+      chain_state_queue := [attacker_call_PassHasBeenSetMsg cstate]
+    |}) in H_exec.
+    simpl in *.
+    destruct(
+      send_or_call attacker attacker caddr 0
+      (Some (serialize (PassHasBeenSetMsg (sha3 attacker_pass))))
+      (add_new_block_to_env (get_valid_header miner s) s)) eqn : H_send_or_call_GetGift;try congruence.
+    unfold send_or_call in  H_send_or_call_GetGift.
+    simpl in H_send_or_call_GetGift.
+    eapply address_not_contract_negb in H_miner.
+    assert( H_caddr_not_EOA : address_is_contract caddr = true).
+    {
+      eapply contract_addr_format in Hec_s;eauto.
+      eapply transition_reachable_impl_reachable in Htrc_s;eauto.  
+    }
+    destruct_address_eq;simpl in *;try congruence.
+    
+    (* 
+      e: sender cstate = miner
+      n: caddr <> sender cstate
+      e0: caddr = caddr
+      n0: caddr <> miner 
+    *)
+
+    destruct(0 >? miner_reward + env_account_balances s attacker)%Z;try congruence.
+    rewrite Hec_s in H_send_or_call_GetGift.
+    assert(Hcstate_s_t0:contract_state s caddr = Some cstate) by eauto.
+    unfold contract_state in Hcstate_s_t0.
+    simpl in Hcstate_s_t0.
+    destruct (env_contract_states s caddr) eqn : Hcstate_s_t0';try congruence.
+    destruct (weak_error_to_error_receive
+    (wc_receive contract
+       (s <| chain_height := S (chain_height s) |> <|
+        current_slot := (current_slot s + 1)%nat |> <|
+        finalized_height := finalized_height s |>)
+       {|
+         ctx_origin := attacker;
+         ctx_from := attacker;
+         ctx_contract_address := caddr;
+         ctx_contract_balance :=
+           0 + env_account_balances s caddr;
+         ctx_amount := 0
+       |} s1
+       (Some
+          (serialize
+             (PassHasBeenSetMsg (sha3 attacker_pass)))))) eqn : H_wc_receive_s1;try congruence.
+    unfold weak_error_to_error_receive in H_wc_receive_s1.
+    unfold bind_error in H_wc_receive_s1.
+    destruct (wc_receive contract
+    (s <| chain_height := S (chain_height s) |> <| current_slot
+     := (current_slot s + 1)%nat |> <| finalized_height :=
+     finalized_height s |>)
+    {|
+      ctx_origin := attacker;
+      ctx_from := attacker;
+      ctx_contract_address := caddr;
+      ctx_contract_balance := 0 + env_account_balances s caddr;
+      ctx_amount := 0
+    |} s1
+    (Some (serialize (PassHasBeenSetMsg (sha3 attacker_pass)))))
+      eqn : H_wc_receive_s1';try congruence.
+    
+    set (cchain := s <| chain_height := S (chain_height s) |> <| current_slot :=
+    (current_slot s + 1)%nat |> <| finalized_height :=
+    finalized_height s |>) in H_wc_receive_s1'.
+    set (cctx := {|
+    ctx_origin := user1;
+    ctx_from := user1;
+    ctx_contract_address := caddr;
+    ctx_contract_balance := 0 + env_account_balances s caddr;
+    ctx_amount := 0
+    |}) in H_wc_receive_s1'.
+    
+    destruct t2 as [new_state new_acts].
+
+    destruct (wc_receive_strong ltac:(try eassumption))
+    as (prev_state_strong & msg_strong & resp_state_strong &
+      deser_state & deser_msg & <- & receive).
+
+    simpl in deser_msg.
+    destruct (msg_strong) eqn : H_msg;try congruence.
+    rewrite deserialize_serialize in deser_msg.
+    rewrite <- deser_msg in receive.
+    rewrite deser_state in Hcstate_s_t0.
+    simpl in receive.
+    rename receive into receive_some.
+    unfold receive in receive_some.
+    reduce_passHasBeenSet_fn.
+    (* 111 *)
+    inversion receive_some.
+    subst.
+    inversion H_wc_receive_s1;subst.
+    inversion H_send_or_call_GetGift;subst.
+    simpl in H_exec.
+    inversion H_exec;subst.
+    inversion Htrans;subst.
+    inversion H_send_or_call_GetGift;subst.
+    inversion Hcs_s';subst.
+    unfold contract_state in H0.
+    simpl in H0.
+    destruct_address_eq;eauto.
+    setoid_rewrite deserialize_serialize in H0.
+    inversion H0.
+    simpl.
+    inversion Hcstate_s_t0.
+    rewrite <- H_pass.
+    intuition.
+    destruct_address_eq;try congruence.
+
+
+
+    (* n: attacker <> miner
+      e: caddr = attacker
+      e0: caddr = caddr
+      n0: caddr <> miner *)
+
+    eapply address_not_contract_negb in attacker_eoa.
+    rewrite e in *.
+    intuition.
+
+    (* 
+      n: attacker <> miner
+    n0: caddr <> attacker
+    e: caddr = caddr
+    n1: caddr <> miner
+    
+    *)
+    destruct(0 >?  env_account_balances s attacker)%Z;try congruence.
+    rewrite Hec_s in H_send_or_call_GetGift.
+    assert(Hcstate_s_t0:contract_state s caddr = Some cstate) by eauto.
+    unfold contract_state in Hcstate_s_t0.
+    simpl in Hcstate_s_t0.
+    destruct (env_contract_states s caddr) eqn : Hcstate_s_t0';try congruence.
+    destruct (weak_error_to_error_receive
+    (wc_receive contract
+       (s <| chain_height := S (chain_height s) |> <|
+        current_slot := (current_slot s + 1)%nat |> <|
+        finalized_height := finalized_height s |>)
+       {|
+         ctx_origin := attacker;
+         ctx_from := attacker;
+         ctx_contract_address := caddr;
+         ctx_contract_balance :=
+           0 + env_account_balances s caddr;
+         ctx_amount := 0
+       |} s1
+       (Some
+          (serialize
+             (PassHasBeenSetMsg (sha3 attacker_pass)))))) eqn : H_wc_receive_s1;try congruence.
+    unfold weak_error_to_error_receive in H_wc_receive_s1.
+    unfold bind_error in H_wc_receive_s1.
+    destruct (wc_receive contract
+    (s <| chain_height := S (chain_height s) |> <| current_slot
+     := (current_slot s + 1)%nat |> <| finalized_height :=
+     finalized_height s |>)
+    {|
+      ctx_origin := attacker;
+      ctx_from := attacker;
+      ctx_contract_address := caddr;
+      ctx_contract_balance := 0 + env_account_balances s caddr;
+      ctx_amount := 0
+    |} s1
+    (Some (serialize (PassHasBeenSetMsg (sha3 attacker_pass)))))
+      eqn : H_wc_receive_s1';try congruence.
+    
+    set (cchain := s <| chain_height := S (chain_height s) |> <| current_slot :=
+    (current_slot s + 1)%nat |> <| finalized_height :=
+    finalized_height s |>) in H_wc_receive_s1'.
+    set (cctx := {|
+    ctx_origin := user1;
+    ctx_from := user1;
+    ctx_contract_address := caddr;
+    ctx_contract_balance := 0 + env_account_balances s caddr;
+    ctx_amount := 0
+    |}) in H_wc_receive_s1'.
+    
+    destruct t2 as [new_state new_acts].
+
+    destruct (wc_receive_strong ltac:(try eassumption))
+    as (prev_state_strong & msg_strong & resp_state_strong &
+      deser_state & deser_msg & <- & receive).
+
+    simpl in deser_msg.
+    destruct (msg_strong) eqn : H_msg;try congruence.
+    rewrite deserialize_serialize in deser_msg.
+    rewrite <- deser_msg in receive.
+    rewrite deser_state in Hcstate_s_t0.
+    simpl in receive.
+    rename receive into receive_some.
+    unfold receive in receive_some.
+    reduce_passHasBeenSet_fn.
+    (* 111 *)
+    inversion receive_some.
+    subst.
+    inversion H_wc_receive_s1;subst.
+    inversion H_send_or_call_GetGift;subst.
+    simpl in H_exec.
+    inversion H_exec;subst.
+    inversion Htrans;subst.
+    inversion H_send_or_call_GetGift;subst.
+    inversion Hcs_s';subst.
+    unfold contract_state in H0.
+    simpl in H0.
+    destruct_address_eq;eauto.
+    setoid_rewrite deserialize_serialize in H0.
+    inversion H0.
+    simpl.
+    inversion Hcstate_s_t0.
+    rewrite <- H_pass.
+    intuition.
+    destruct_address_eq;try congruence.
+  Qed.
+
+  Require stdpp.countable.
+
+  Lemma tmp:
+    exists tr s (tr' : TransitionTrace miner s0 s)  cstate,
+    interleavedExecution miner [honest] honest_strat [attacker] attacker_strat s0 s0 tr Tusr s tr' /\
+    contract_state s caddr = Some cstate /\
+    cstate.(passHasBeenSet) = true /\
+    cstate.(hashPass) <> sha3 honest_pass /\
+    funds s caddr > 0.
+  Proof.
+    assert (tr0 : TransitionTrace miner s0 s0) by eapply clnil.
+    decompose_is_init_state H_init.
+    simpl in *.
+    reduce_init.
+    unfold negb in Einit.
+    destruct (setup_passHasBeenSet setup) eqn : H_passBset;try congruence.
+    assert (exists s' , transition miner s0 (attacker_call_SetPass state) = Ok s').
+    {
+      eapply attacker_call_SetPass_is_call_act_transition_correct.
+      unfold contract_state.
+      rewrite H_env_states.
+      simpl.
+      setoid_rewrite deserialize_serialize.
+      eauto.
+      unfold transition_reachable.
+      split.
+      eauto.
+      econstructor;eauto.
+      inversion H_init0.
+      simpl.
+      eauto.
+    }
+    destruct H as [s' Htrans].
+    eapply attacker_call_SetPass_is_call_act_state_correct in Htrans as Ht.
+    destruct Ht as [Hcs_s' [Hhash Hset]].
+    assert (Hcall : is_call_act (attacker_call_SetPass state) = true).
+    {
+      eapply attacker_call_SetPass_is_call_act.
+    }
+
+    set (tr_s' := snoc tr0 (step_trans miner (attacker_call_SetPass state) Hcall Htrans) ).
+
+    assert (exists s'' , transition miner s' (attacker_call_PassHasBeenSetMsg Hcs_s') = Ok s'').
+    {
+      eapply attacker_call_PassHasBeenSetMsg_is_call_act_transition_correct.
+      eauto.
+      unfold contract_state.
+      unfold transition_reachable.
+      split.
+      eauto.
+      econstructor;eauto.
+      eauto.
+      inversion H_init0.
+      simpl.
+      destruct Hset.
+      eauto.
+      destruct Hset.
+      eauto.
+    }
+    destruct H as [s'' Htrans''].
+    eapply attacker_call_PassHasBeenSetMsg_is_call_act_state_correct in Htrans'' as Ht'.
+    destruct Ht' as [Hcs_s'' [Hhash' Hset']].
+    assert (Hcall' : is_call_act (attacker_call_PassHasBeenSetMsg Hcs_s') = true).
+    {
+      eapply attacker_call_PassHasBeenSetMsg_is_call_act.
+    }
+    set (tr_s'' := snoc tr_s' (step_trans miner (attacker_call_PassHasBeenSetMsg Hcs_s') Hcall' Htrans'') ).
+    exists tr0.
+    exists s''.
+    exists tr_s''.
+    exists Hcs_s''.
+    split.
+    assert (interleavedExecution miner [honest] honest_strat [attacker] attacker_strat s0
+    s0 tr0 Tenv s0 tr0).
+    {
+      eapply IS_Refl.
+    }
+    (* stratDrive  addrs_usr delta_usr s0  s' tr' s'' tr'' *)
+    assert (stratDrive miner [attacker] attacker_strat s0 s0 tr0 s' tr_s').
+    {
+      unfold stratDrive.
+      exists (attacker_call_SetPass state).
+      exists Hcall.
+      exists Htrans.
+      split;eauto.
+      unfold attacker_strat.
+      simpl.
+      unfold get_contract_state.
+      rewrite H_env_states.
+      setoid_rewrite deserialize_serialize.
+      destruct ((hashPass state =? sha3 attacker_pass)%N) eqn : Ht.
+      + inversion H_init0;subst.
+        simpl in *.
+        congruence.
+      + destruct (passHasBeenSet state) eqn : Ht'.
+        - inversion H_init0;subst.
+          simpl in *.
+          congruence.
+        - simpl.
+          eauto.
+    }
+    assert (stratDrive miner [attacker] attacker_strat s0 s' tr_s' s'' tr_s'').
+    {
+      unfold stratDrive.
+      exists (attacker_call_PassHasBeenSetMsg Hcs_s').
+      exists Hcall'.
+      exists Htrans''.
+      split;eauto.
+      unfold attacker_strat.
+      simpl.
+      unfold get_contract_state.
+      unfold contract_state in Hhash.
+      destruct (env_contract_states s' caddr) eqn : Hcstate_s';try congruence.
+      simpl in *.
+      rewrite Hhash.
+      destruct Hset.
+      rewrite H1.
+      destruct ((sha3 attacker_pass =? sha3 attacker_pass)%N) eqn : Ht;try congruence.
+      +  eauto.
+        simpl.
+        eauto.
+      + eapply Pos.eqb_neq in Ht.
+        unfold not in Ht.
+        assert (countable.encode attacker_pass = countable.encode attacker_pass).
+        {
+        eapply stdpp.countable.encode_inj.
+        eauto.
+        }
+        intuition.
+      + simpl in  Hhash.
+        congruence.
+    }
+    assert(multiStratDrive miner [attacker] attacker_strat s0 s0 tr0  s0 tr0 0) by eapply MS_Refl.
+    assert(multiStratDrive miner [attacker] attacker_strat s0 s0 tr0  s' tr_s' 1).
+    {
+      eapply MS_Step in H2;eauto.
+    }
+    assert(multiStratDrive miner [attacker] attacker_strat s0 s0 tr0  s'' tr_s'' 2).
+    {
+      eapply MS_Step in H3;eauto.
+    }
+
+    eapply ISE_Step in H4;eauto.
+    split.
+    eauto.
+    split.
+    destruct Hset'.
+    eauto.
+    split.
+    destruct Hset'.
+    rewrite H.
+    eauto.
+    unfold sha3.
+    unfold not.
+    intros.
+    inversion H1.
+    eapply stdpp.countable.encode_inj in H3.
+    congruence.
+    eapply attacker_call_PassHasBeenSetMsg_is_call_act_state_correct_funds in Htrans'' as Ht.
+    eapply attacker_call_SetPass_is_call_act_state_correct_funds in Htrans as Ht'.
+    lia.
+    unfold contract_state.
+    rewrite H_env_states.
+    simpl.
+    setoid_rewrite deserialize_serialize.
+    eauto.
+    unfold transition_reachable.
+    split.
+    eauto.
+    econstructor;eauto.
+    inversion H_init0.
+    simpl.
+    eauto.
+    eauto.
+    unfold transition_reachable.
+    split.
+    eauto.
+    econstructor;eauto.
+    destruct Hset.
+    eauto.
+    destruct Hset.
+    eauto.
+    eauto.
+    unfold transition_reachable.
+    split.
+    eauto.
+    econstructor;eauto.
+    destruct Hset.
+    eauto.
+    destruct Hset.
+    eauto.
+    eauto.
+    unfold transition_reachable.
+    unfold contract_state.
+    rewrite H_env_states.
+    simpl.
+    setoid_rewrite deserialize_serialize.
+    eauto.
+    unfold transition_reachable.
+    split.
+    eauto.
+    econstructor;eauto.
+    inversion H_init0.
+    simpl.
+    eauto.
+  Qed.
+  
 End Liqiuidity.
 
